\let\negmedspace\undefined
\let\negthickspace\undefined
\documentclass[journal,12pt,twocolumn]{IEEEtran}
\usepackage[utf8]{inputenc}
\usepackage{amsmath}
\usepackage{amssymb}
 \usepackage{polynom}
\usepackage{listings}
\lstset{
frame=single, 
breaklines=true,
columns=fullflexible
}

\title{AI1110 assignment 2 

ICSE 12 2017}
\author{Pranav Pettugadi

CS21BTECH11063}
\date{April 2022}

\begin{document}
\bibliographystyle{IEEEtran}

\providecommand{\brak}[1]{\ensuremath{\left(#1\right)}}
\providecommand{\lbrak}[1]{\ensuremath{\left(#1\right.}}
\providecommand{\rbrak}[1]{\ensuremath{\left.#1\right)}}

\newcommand{\question}{\noindent \textbf{Question: }}	
\newcommand{\solution}{\noindent \textbf{Solution: }}
\maketitle
\question {1(iii)} prove that $$\frac{1}{2}\cos^{-1}\brak{\frac{1-x}{1+x}} = \tan^{-1}{\sqrt{x}}$$

\solution
let$$ x= tan^2(y)$$

\begin{align*}
\implies&\frac{1}{2}\cos^{-1}\brak{\frac{1-x}{1+x}}\\
\implies&\frac{1}{2}\cos^{-1}\brak{\frac{1-tan^2(y)}{1+tan^2(y)}}\\\
\implies&\frac{1}{2}\cos^{-1}({\cos{2y}})\\
\implies&\frac{1}{2} 2y\\
\implies&y\\
\implies&tan^{-1}\sqrt{x}\\
\end{align*}

$\therefore$ $\frac{1}{2}\cos^{-1}\brak{\frac{1-x}{1+x}} = \tan^{-1}{\sqrt{x}}$

\end{document}
